Polishing

Uniswap_Pool.thy
@@ -7,9 +7,9 @@ no_notation Reals ("\<real>") (*TODO: use that patch!*)
 type_synonym fee_protocol = \<open>nat \<times> nat\<close>
 
 datatype pool = pool (price: real) (tick: int) (unlocked: bool) (liquidity: real)
-                     (growth: growth) (fee_protocol: fee_protocol) (protocal_fees: \<open>fee \<times> fee\<close>)
+                     (growth: growth) (fee_protocol: fee_protocol) (protocol_fees: \<open>fee \<times> fee\<close>)
 
-hide_const (open) price tick unlocked liquidity growth fee_protocol protocal_fees
+hide_const (open) price tick unlocked liquidity growth fee_protocol protocol_fees
 
 setup \<open>Sign.mandatory_path "pool"\<close>
 
@@ -56,8 +56,8 @@ lemma [\<phi>reason 1000]: \<open> Is_Literal fee\<close> unfolding Is_Literal_d
 
 proc (nodef) fee[\<phi>synthesis 1100]:
   input \<open>Void\<close>
-  output \<open>fee \<Ztypecolon> \<v>\<a>\<l> \<real>\<close>
-  \<medium_left_bracket> op_const_areal[where x=fee] \<medium_right_bracket>. .
+  output \<open>fee_rate \<Ztypecolon> \<v>\<a>\<l> \<real>\<close>
+  \<medium_left_bracket> op_const_areal[where x=fee_rate] \<medium_right_bracket>. .
 
 
 locale Pool = Tickmap_spec + Tick_spec +
@@ -112,11 +112,11 @@ locale Pool = Tickmap_spec + Tick_spec +
   and get_fee_protocol_1[\<phi>synthesis 1000]:
     \<open> \<p>\<r>\<o>\<c> op_get_fee_protocol_1 \<lbrace> s \<Ztypecolon> Pool \<longmapsto> s \<Ztypecolon> Pool\<heavy_comma> snd (pool.fee_protocol s) \<Ztypecolon> \<v>\<a>\<l> \<nat> \<rbrace> \<close>
   and get_pool_protocal_fee_0_\<phi>app[\<phi>synthesis 1000]:
-    \<open> \<p>\<r>\<o>\<c> op_get_protocal_fee_0 \<lbrace> s \<Ztypecolon> Pool \<longmapsto> s \<Ztypecolon> Pool\<heavy_comma> fst (pool.protocal_fees s) \<Ztypecolon> \<v>\<a>\<l> \<real> \<rbrace> \<close>
+    \<open> \<p>\<r>\<o>\<c> op_get_protocal_fee_0 \<lbrace> s \<Ztypecolon> Pool \<longmapsto> s \<Ztypecolon> Pool\<heavy_comma> fst (pool.protocol_fees s) \<Ztypecolon> \<v>\<a>\<l> \<real> \<rbrace> \<close>
   and set_pool_protocal_fee_0_\<phi>app:
     \<open> \<p>\<r>\<o>\<c> op_set_protocal_fee_0 rv \<lbrace> s \<Ztypecolon> Pool\<heavy_comma> c' \<Ztypecolon> \<v>\<a>\<l>[rv] \<real> \<longmapsto> pool.map_protocal_fees (apfst (\<lambda>_. c')) s \<Ztypecolon> Pool \<rbrace> \<close>
   and get_pool_protocal_fee_1_\<phi>app[\<phi>synthesis 1000]:
-    \<open> \<p>\<r>\<o>\<c> op_get_protocal_fee_1 \<lbrace> s \<Ztypecolon> Pool \<longmapsto> s \<Ztypecolon> Pool\<heavy_comma> snd (pool.protocal_fees s) \<Ztypecolon> \<v>\<a>\<l> \<real> \<rbrace> \<close>
+    \<open> \<p>\<r>\<o>\<c> op_get_protocal_fee_1 \<lbrace> s \<Ztypecolon> Pool \<longmapsto> s \<Ztypecolon> Pool\<heavy_comma> snd (pool.protocol_fees s) \<Ztypecolon> \<v>\<a>\<l> \<real> \<rbrace> \<close>
   and set_pool_protocal_fee_1_\<phi>app:
     \<open> \<p>\<r>\<o>\<c> op_set_protocal_fee_1 rv \<lbrace> s \<Ztypecolon> Pool\<heavy_comma> c' \<Ztypecolon> \<v>\<a>\<l>[rv] \<real> \<longmapsto> pool.map_protocal_fees (apsnd (\<lambda>_. c')) s \<Ztypecolon> Pool \<rbrace> \<close>
 
@@ -125,9 +125,9 @@ begin
 
 definition Uniswap_Pool :: \<open>(fiction, price \<times> tick \<times> bool \<times> liquiditys \<times> liquiditys \<times> growths \<times> opt_growths \<times> fee_protocol \<times> (fee \<times> fee)) \<phi>\<close>
   where [\<phi>defs]: \<open>Uniswap_Pool x = (
-    case x of (price, i, unlocked, Lg, L, growth, \<delta>, fee_proto, protocal_fees) \<Rightarrow>
+    case x of (price, i, unlocked, Lg, L, growth, \<delta>, fee_proto, protocol_fees) \<Rightarrow>
         \<comment> \<open>\<open>growth\<close> is the abstract growth happened on every tick\<close>
-      pool price i unlocked (L i) (gSum growth) fee_proto protocal_fees \<Ztypecolon> Pool\<heavy_comma>
+      pool price i unlocked (L i) (gSum growth) fee_proto protocol_fees \<Ztypecolon> Pool\<heavy_comma>
         \<comment> \<open>so the global fee growth is the sum of the \<open>growth\<close> over every tick\<close>
       (\<lambda>k. 0 < Lg k) \<Ztypecolon> Tickmap\<heavy_comma>
         \<comment> \<open>\<open>k \<in> dom \<delta>\<close> means the tick \<open>k\<close> is initialized\<close>
@@ -138,8 +138,8 @@ definition Uniswap_Pool :: \<open>(fiction, price \<times> tick \<times> bool \<
 declare [[\<phi>trace_reasoning = 1]]
 
 lemma [\<phi>reason 1200]:
-  \<open>(price, i, unlocked, Lg, L, growth, \<delta>, fee_proto, protocal_fees) \<Ztypecolon> Uniswap_Pool \<i>\<m>\<p>\<l>\<i>\<e>\<s>
-   pool price i unlocked (L i) (gSum growth) fee_proto protocal_fees \<Ztypecolon> Pool\<heavy_comma>
+  \<open>(price, i, unlocked, Lg, L, growth, \<delta>, fee_proto, protocol_fees) \<Ztypecolon> Uniswap_Pool \<i>\<m>\<p>\<l>\<i>\<e>\<s>
+   pool price i unlocked (L i) (gSum growth) fee_proto protocol_fees \<Ztypecolon> Pool\<heavy_comma>
    (\<lambda>k. 0 < Lg k) \<Ztypecolon> Tickmap\<heavy_comma>
    (Lg, L, growth, i, \<delta>) \<Ztypecolon> Ticks
   \<a>\<n>\<d> (tick_of_price price = i \<or> price = price_of (i + 1))
@@ -148,14 +148,14 @@ lemma [\<phi>reason 1200]:
 
 lemma [\<phi>reason 100]:
   \<open> \<p>\<r>\<e>\<m>\<i>\<s>\<e> (tick_of_price price = i \<or> price = price_of (i + 1))
-\<Longrightarrow> X \<i>\<m>\<p>\<l>\<i>\<e>\<s> pool price i unlocked (L i) (gSum growth) fee_proto protocal_fees \<Ztypecolon> Pool\<heavy_comma>
+\<Longrightarrow> X \<i>\<m>\<p>\<l>\<i>\<e>\<s> pool price i unlocked (L i) (gSum growth) fee_proto protocol_fees \<Ztypecolon> Pool\<heavy_comma>
         (\<lambda>k. 0 < Lg k) \<Ztypecolon> Tickmap\<heavy_comma>
         (Lg, L, growth, i, \<delta>) \<Ztypecolon> Ticks \<r>\<e>\<m>\<a>\<i>\<n>\<s> R \<a>\<n>\<d> P
-\<Longrightarrow> X \<i>\<m>\<p>\<l>\<i>\<e>\<s> (price, i, unlocked, Lg, L, growth, \<delta>, fee_proto, protocal_fees) \<Ztypecolon> Uniswap_Pool \<r>\<e>\<m>\<a>\<i>\<n>\<s> R \<a>\<n>\<d> P\<close>
+\<Longrightarrow> X \<i>\<m>\<p>\<l>\<i>\<e>\<s> (price, i, unlocked, Lg, L, growth, \<delta>, fee_proto, protocol_fees) \<Ztypecolon> Uniswap_Pool \<r>\<e>\<m>\<a>\<i>\<n>\<s> R \<a>\<n>\<d> P\<close>
   unfolding FOCUS_TAG_def
   \<medium_left_bracket> premises _ and I
     I 
-    construct\<phi> \<open>(price, i, unlocked, Lg, L, growth, \<delta>, fee_proto, protocal_fees) \<Ztypecolon> Uniswap_Pool\<close>
+    construct\<phi> \<open>(price, i, unlocked, Lg, L, growth, \<delta>, fee_proto, protocol_fees) \<Ztypecolon> Uniswap_Pool\<close>
   \<medium_right_bracket>. .
 
 declare Invt_Ticks_def[simp] Invt_A_Tick_def[simp]
@@ -172,14 +172,14 @@ definition swap_loop_transition :: \<open>bool \<Rightarrow> bool \<Rightarrow> 
 definition \<open>\<Delta>protocal_fees fee_proto zeroForOne L price price' \<gamma>
     = (if zeroForOne
        then if 0 < fst fee_proto
-            then (fst (reserve_change zeroForOne L price price') * fee_factor / real (fst fee_proto), 0)
+            then (fst (reserve_change zeroForOne L price price') * fee_rate' / real (fst fee_proto), 0)
             else (0,0)
        else if 0 < snd fee_proto
-            then (0, snd (reserve_change zeroForOne L price price') * fee_factor / real (snd fee_proto))
+            then (0, snd (reserve_change zeroForOne L price price') * fee_rate' / real (snd fee_proto))
             else (0,0))\<close>
 
 proc swap:
-  input \<open>(price, i, unlocked, Lg, L, growth, \<delta>, fee_protocol, protocal_fees) \<Ztypecolon> Uniswap_Pool\<heavy_comma>
+  input \<open>(price, i, unlocked, Lg, L, growth, \<delta>, fee_protocol, protocol_fees) \<Ztypecolon> Uniswap_Pool\<heavy_comma>
          zeroForOne \<Ztypecolon> \<v>\<a>\<l> \<bool>\<heavy_comma> amount_specified \<Ztypecolon> \<v>\<a>\<l> \<real>\<heavy_comma> price_limit \<Ztypecolon> \<v>\<a>\<l> \<real>\<close>
   premises \<open>0 \<noteq> amount_specified \<and> 0 < price_limit\<close> and \<open>unlocked\<close>
       and \<open>if zeroForOne then price_limit < price \<and> price_limit > MIN_PRICE
@@ -187,15 +187,15 @@ proc swap:
     (*soon we will not need to declare these pre-conditions but verify that
         a revert will happen once they are violated*)
   output \<open>(price', i', unlocked, Lg, L,
-            growth + fee_growth zeroForOne fee_factor L price price',
+            growth + fee_growth zeroForOne fee_rate' L price price',
             \<delta>, fee_protocol,
-            protocal_fees + \<Delta>protocal_fees fee_protocol zeroForOne L price price' fee_factor) \<Ztypecolon> Uniswap_Pool\<heavy_comma>
+            protocol_fees + \<Delta>protocal_fees fee_protocol zeroForOne L price price' fee_rate') \<Ztypecolon> Uniswap_Pool\<heavy_comma>
           transfer_out \<Ztypecolon> \<v>\<a>\<l> \<real>\<heavy_comma> transfer_in \<Ztypecolon> \<v>\<a>\<l> \<real>
     \<s>\<u>\<b>\<j> price' i' transfer_out transfer_in.
       (if zeroForOne then price_limit \<le> price' else price' \<le> price_limit) \<and>
       (price' = price_limit \<or> (
       if 0 < amount_specified
-      then amount_specified * (1 - fee) = (if zeroForOne then fst else snd) (reserve_change zeroForOne L price price')
+      then amount_specified * (1 - fee_rate) = (if zeroForOne then fst else snd) (reserve_change zeroForOne L price price')
       else - amount_specified = (if zeroForOne then snd else fst) (reserve_change zeroForOne L price price') ))
       \<comment> \<open>The resulted price either reaches the price limit, or, is the one having a reserve change
              meeting the specified amount.
@@ -205,10 +205,10 @@ proc swap:
           which is, \<open>i'\<close> is the tick of the \<open>price'\<close>, \<open>price_of i' \<le> price \<le> price_of (i' + 1)\<close>\<close>
       \<comment> \<open>Gross liquidity \<open>Lg\<close>, actual liquidity \<open>L\<close>, the absolute difference \<open>\<delta>\<close> in recorded fee growth,
           and the proportion \<open>fee_protocol\<close> of the protocol fee, are not changed\<close>
-      \<comment> \<open>The fee growth \<open>growth + fee_growth zeroForOne fee_factor L price price'\<close>
-          and the \<open>protocal_fees\<close> are increased accordingly.\<close>
+      \<comment> \<open>The fee growth \<open>growth + fee_growth zeroForOne fee_rate' L price price'\<close>
+          and the \<open>protocol_fees\<close> are increased accordingly.\<close>
    \<and> transfer_out = (if zeroForOne then snd else fst) (reserve_change zeroForOne L price price')
-   \<and> transfer_in = (if zeroForOne then fst else snd) (reserve_change zeroForOne L price price') / (1 - fee)
+   \<and> transfer_in = (if zeroForOne then fst else snd) (reserve_change zeroForOne L price price') / (1 - fee_rate)
     \<comment> \<open>As \<phi>-system hasn't formalized transfer and external call, we cannot verify the last transfer operation
       in the swap function, but only verify the amount of transfer-out and that of transfer-in. \<close>
 \<close>
@@ -251,8 +251,8 @@ proc swap:
            pf \<Ztypecolon> \<v>\<a>\<r>[\<v>\<a>\<r>_protocolFee] \<real>\<heavy_comma>
             j \<Ztypecolon> \<v>\<a>\<r>[\<v>\<a>\<r>_tick] Tick\<heavy_comma>
            L j \<Ztypecolon> \<v>\<a>\<r>[\<v>\<a>\<r>_liquidity] \<real>\<heavy_comma>
-          I_fee_growth_global (growth + fee_growth zeroForOne fee_factor L price pr) \<Ztypecolon> \<v>\<a>\<r>[\<v>\<a>\<r>_fee_growth_global] \<real>\<heavy_comma>
-          (Lg, L, growth + fee_growth zeroForOne fee_factor L price pr, j, \<delta>) \<Ztypecolon> Ticks
+          I_fee_growth_global (growth + fee_growth zeroForOne fee_rate' L price pr) \<Ztypecolon> \<v>\<a>\<r>[\<v>\<a>\<r>_fee_growth_global] \<real>\<heavy_comma>
+          (Lg, L, growth + fee_growth zeroForOne fee_rate' L price pr, j, \<delta>) \<Ztypecolon> Ticks
         \<s>\<u>\<b>\<j> ar pr ac pf j.
             Inv: ( MIN_PRICE \<le> pr \<and> pr < MAX_PRICE
                  \<and> j < MAX_TICK
@@ -261,9 +261,9 @@ proc swap:
                  \<and> (let (\<Delta>reserve0, \<Delta>reserve1) = reserve_change zeroForOne L price pr;
                         amountIn = (if zeroForOne then \<Delta>reserve0 else \<Delta>reserve1) ;
                         amountOut = (if zeroForOne then \<Delta>reserve1 else \<Delta>reserve0)
-                     in (if ?exactInput then amount_specified - amountIn / (1 - fee) else amount_specified + amountOut) = ar
-                      \<and> (if ?exactInput then - amountOut else amountIn / (1 - fee)) = ac
-                      \<and> (if 0 < fee_proto then amountIn * fee / (1-fee) / real fee_proto else 0) = pf
+                     in (if ?exactInput then amount_specified - amountIn / (1 - fee_rate) else amount_specified + amountOut) = ar
+                      \<and> (if ?exactInput then - amountOut else amountIn / (1 - fee_rate)) = ac
+                      \<and> (if 0 < fee_proto then amountIn * fee_rate' / real fee_proto else 0) = pf
                    )
                  
           )
@@ -279,7 +279,7 @@ proc swap:
         if \<open>$tick_next > MAX_TICK\<close> \<medium_left_bracket> \<open>MAX_TICK\<close> \<rightarrow> tick_next \<medium_right_bracket>. \<medium_left_bracket> \<medium_right_bracket>. ;;
       \<medium_right_bracket>. as \<open>tick_next \<Ztypecolon> Tick\<close> affirm unfolding tick_next_def using \<phi> by auto ;;
 
-      let ?growth' = \<open>growth + fee_growth zeroForOne fee_factor L price pr\<close>
+      let ?growth' = \<open>growth + fee_growth zeroForOne fee_rate' L price pr\<close>
 
       have t0[useful]: \<open>0 < pr\<close> by (smt (verit) the_\<phi>(25) the_\<phi>(3) the_\<phi>(33))
 
@@ -331,30 +331,30 @@ proc swap:
         fee)
         \<exists>next_price, amountIn, amountOut, fee_amount
      \<rightarrow> val amountIn, amountOut, feeAmount \<rightarrow> price ;;
-     (*FIX ME: ^ there is a bug*)
+     (*FIX ME: ^ there is a bug in programming system*)
 
-      have d2: \<open>fee_amount = amountIn * fee_factor\<close> unfolding fee_factor_def using swap_step_fee_amout the_\<phi>(19) by force
+      have d2: \<open>fee_amount = amountIn * fee_rate'\<close> unfolding fee_rate'_def using swap_step_fee_amout the_\<phi>(19) by force
 
-      have d1[simp]: \<open>amountIn + fee_amount = amountIn / (1 - fee)\<close> by (smt (verit, ccfv_threshold) ab_semigroup_mult_class.mult_ac(1) add.commute add_diff_cancel_left' cancel_comm_monoid_add_class.diff_cancel comm_semiring_class.distrib d2 diff_add_eq diff_diff_eq2 diff_zero div_by_1 divide_cancel_right divide_divide_eq_left divide_divide_eq_left' divide_divide_eq_right divide_eq_0_iff divide_real_def eq_divide_imp fee_range linorder_not_le minus_diff_eq mult.commute mult.left_commute mult.right_neutral mult_1 mult_cancel_left2 mult_eq_0_iff mult_zero_left mult_zero_right nle_le nonzero_divide_mult_cancel_left nonzero_mult_div_cancel_left order_refl real_divide_square_eq right_diff_distrib' ring_class.ring_distribs(1) times_divide_eq_left fee_factor_def)
+      have d1[simp]: \<open>amountIn + fee_amount = amountIn / (1 - fee_rate)\<close> by (smt (verit, ccfv_threshold) ab_semigroup_mult_class.mult_ac(1) add.commute add_diff_cancel_left' cancel_comm_monoid_add_class.diff_cancel comm_semiring_class.distrib d2 diff_add_eq diff_diff_eq2 diff_zero div_by_1 divide_cancel_right divide_divide_eq_left divide_divide_eq_left' divide_divide_eq_right divide_eq_0_iff divide_real_def eq_divide_imp fee_rate_range linorder_not_le minus_diff_eq mult.commute mult.left_commute mult.right_neutral mult_1 mult_cancel_left2 mult_eq_0_iff mult_zero_left mult_zero_right nle_le nonzero_divide_mult_cancel_left nonzero_mult_div_cancel_left order_refl real_divide_square_eq right_diff_distrib' ring_class.ring_distribs(1) times_divide_eq_left fee_rate'_def)
 
       have t1[simp]: \<open>L j = 0 \<Longrightarrow> fee_amount = 0\<close> using \<open>_ = swap_step _ _ _ _ _\<close> by (auto simp add: swap_step_def Let_def)
 
       have kk1: \<open>MIN_PRICE < (if zeroForOne then max ?step_price_next price_limit else min ?step_price_next price_limit)\<close> using price_of_smono the_\<phi>(24) the_\<phi>(27) the_\<phi>(31) the_\<phi>(33) the_\<phi>lemmata(2) x1' by force
 
-      have kk2: \<open>MIN_PRICE < next_price\<close> using fee_range kk1 swap_step_next_price_Le_MIN_PRICE the_\<phi>(16) the_\<phi>(25) the_\<phi>(31) the_\<phi>lemmata(5) by blast
+      have kk2: \<open>MIN_PRICE < next_price\<close> using fee_rate_range kk1 swap_step_next_price_Le_MIN_PRICE the_\<phi>(16) the_\<phi>(25) the_\<phi>(31) the_\<phi>lemmata(5) by blast
 
-      have kk4: \<open>\<not> zeroForOne \<Longrightarrow> next_price < MAX_PRICE\<close> by (smt (verit, best) fee_range price_of_L0 swap_step_next_price_Gt t0 the_\<phi>(16) the_\<phi>(25) the_\<phi>(27) the_\<phi>(33) the_\<phi>lemmata(5))
+      have kk4: \<open>\<not> zeroForOne \<Longrightarrow> next_price < MAX_PRICE\<close> by (smt (verit, best) fee_rate_range price_of_L0 swap_step_next_price_Gt t0 the_\<phi>(16) the_\<phi>(25) the_\<phi>(27) the_\<phi>(33) the_\<phi>lemmata(5))
         
-      have kk8: \<open>zeroForOne \<Longrightarrow> next_price \<le> pr\<close> by (smt (verit, best) fee_range price_of_L0 price_of_smono price_of_tick swap_step_next_price_LE_price t0 the_\<phi>(16) the_\<phi>(27) the_\<phi>(28) the_\<phi>lemmata(5) x1) 
+      have kk8: \<open>zeroForOne \<Longrightarrow> next_price \<le> pr\<close> by (smt (verit, best) fee_rate_range price_of_L0 price_of_smono price_of_tick swap_step_next_price_LE_price t0 the_\<phi>(16) the_\<phi>(27) the_\<phi>(28) the_\<phi>lemmata(5) x1) 
 
-      have kk6: \<open>zeroForOne \<Longrightarrow> price_of tick_next \<le> next_price \<and> price_limit \<le> next_price\<close> by (smt (verit, best) fee_range kk8 price_of_L0 swap_step_next_price_Le swap_step_next_price_Le_0 t0 the_\<phi>(16) the_\<phi>(25) the_\<phi>lemmata(5))
+      have kk6: \<open>zeroForOne \<Longrightarrow> price_of tick_next \<le> next_price \<and> price_limit \<le> next_price\<close> by (smt (verit, best) fee_rate_range kk8 price_of_L0 swap_step_next_price_Le swap_step_next_price_Le_0 t0 the_\<phi>(16) the_\<phi>(25) the_\<phi>lemmata(5))
         
-      have kk9: \<open>\<not> zeroForOne \<Longrightarrow> pr \<le> next_price\<close> by (smt (verit, ccfv_SIG) fee_range price_of_mono price_of_tick swap_step_next_price_Le swap_step_price_target_LE_next_price t0 the_\<phi>(16) the_\<phi>(25) the_\<phi>(27) the_\<phi>(28) the_\<phi>lemmata(5) x1') 
+      have kk9: \<open>\<not> zeroForOne \<Longrightarrow> pr \<le> next_price\<close> by (smt (verit, ccfv_SIG) fee_rate_range price_of_mono price_of_tick swap_step_next_price_Le swap_step_price_target_LE_next_price t0 the_\<phi>(16) the_\<phi>(25) the_\<phi>(27) the_\<phi>(28) the_\<phi>lemmata(5) x1') 
 
       have kk7: \<open>\<not> zeroForOne \<Longrightarrow> next_price \<le> price_of tick_next \<and> next_price \<le> price_limit\<close>
         apply (auto)
-        apply (smt (verit, ccfv_threshold) fee_range kk9 price_of_L0 swap_step_next_price_Gt t0 the_\<phi>(16) the_\<phi>(25) the_\<phi>(27) the_\<phi>lemmata(5))
-        by (smt (verit, ccfv_SIG) fee_range price_of_L0 swap_step_next_price_LE_price swap_step_next_price_LE_price_target t0 the_\<phi>(16) the_\<phi>(27) the_\<phi>lemmata(5))
+        apply (smt (verit, ccfv_threshold) fee_rate_range kk9 price_of_L0 swap_step_next_price_Gt t0 the_\<phi>(16) the_\<phi>(25) the_\<phi>(27) the_\<phi>lemmata(5))
+        by (smt (verit, ccfv_SIG) fee_rate_range price_of_L0 swap_step_next_price_LE_price swap_step_next_price_LE_price_target t0 the_\<phi>(16) the_\<phi>(27) the_\<phi>lemmata(5))
 
       have ka1: \<open>zeroForOne \<Longrightarrow> \<forall>k. tick_of_price next_price < k \<and> k < tick_of_price pr \<longrightarrow> Lg k = 0\<close> by (metis dual_order.strict_trans2 kk6 order.strict_iff_not price_of_L0 t8 the_\<phi>(28) tick_of_price tick_of_price_LE_mono zle_add1_eq_le)
 
@@ -367,7 +367,7 @@ proc swap:
         by (smt (verit) kk7 price_of_smono price_of_tick t0 t11 the_\<phi>(28))
 
       have p1: \<open>zeroForOne \<Longrightarrow> L (tick_of_price next_price) = L j\<close>
-        by (smt (verit, ccfv_SIG) fee_range kk6 price_of_smono price_of_tick swap_step_next_price_Gt t7 the_\<phi>(16) the_\<phi>(19) the_\<phi>(24) the_\<phi>(25) the_\<phi>(27) the_\<phi>(28) the_\<phi>(35) x1)
+        by (smt (verit, ccfv_SIG) fee_rate_range kk6 price_of_smono price_of_tick swap_step_next_price_Gt t7 the_\<phi>(16) the_\<phi>(19) the_\<phi>(24) the_\<phi>(25) the_\<phi>(27) the_\<phi>(28) the_\<phi>(35) x1)
 
       have p2: \<open>if zeroForOne then (amountIn, amountOut) = reserve_change_in_a_step (L (tick_of_price next_price)) next_price pr
                               else (amountOut, amountIn) = reserve_change_in_a_step (L (tick_of_price pr)) pr next_price\<close>
@@ -398,12 +398,12 @@ proc swap:
       \<medium_right_bracket>. \<medium_left_bracket> \<medium_right_bracket>. ;;
 
       define step_growth where \<open>step_growth = (if L j = 0 then 0 else fee_amount / L j)\<close>
-      define \<Delta>growth where \<open>\<Delta>growth = fee_growth zeroForOne fee_factor L pr next_price\<close> 
+      define \<Delta>growth where \<open>\<Delta>growth = fee_growth zeroForOne fee_rate' L pr next_price\<close> 
 
-      have ak1: \<open>0 < L j \<Longrightarrow> zeroForOne \<Longrightarrow> global_fee0_growth (fee_growth' True fee_factor L next_price pr) = (1/next_price - 1/pr) * fee_factor\<close>
+      have ak1: \<open>0 < L j \<Longrightarrow> zeroForOne \<Longrightarrow> global_fee0_growth (fee_growth' True fee_rate' L next_price pr) = (1/next_price - 1/pr) * fee_rate'\<close>
         using gSum_fee_growth kb1 kk2 kk8 the_\<phi>(30) by force
 
-      have ak2: \<open>0 < L j \<Longrightarrow> \<not> zeroForOne \<Longrightarrow> global_fee1_growth (fee_growth' False fee_factor L pr next_price) = (next_price - pr) * fee_factor\<close>
+      have ak2: \<open>0 < L j \<Longrightarrow> \<not> zeroForOne \<Longrightarrow> global_fee1_growth (fee_growth' False fee_rate' L pr next_price) = (next_price - pr) * fee_rate'\<close>
         using gSum_fee_growth growth.fee1 kb2 kk4 kk9 the_\<phi>(31) by presburger
         
       ;;
@@ -454,8 +454,8 @@ proc swap:
                       using fee_growth_eq_0 kk4 kk9 the_\<phi>(30) the_\<phi>(33) apply auto[1]
                       by (smt (verit, best) fee_growth_eq_0 kk4 kk9 the_\<phi>(20) the_\<phi>(33) tick_of_price) ;;
               affirm unfolding \<Delta>growth_def apply auto
-                    using fee_factor_GT_0 fee_growth_always_ge_0 kk8 the_\<phi>(20) apply force
-                    using fee_factor_GT_0 fee_growth_always_ge_0 kk9 t0 by force ;;
+                    using fee_rate'_GT_0 fee_growth_always_ge_0 kk8 the_\<phi>(20) apply force
+                    using fee_rate'_GT_0 fee_growth_always_ge_0 kk9 t0 by force ;;
               affirm by (auto simp add: prod_eq_iff growth.fee1_def growth.fee0_def) ;; 
             \<rightarrow> var liquidityNet
             \<open>_ \<Ztypecolon> Ticks\<close> is \<open>(_,_, ?growth' + \<Delta>growth, real_next_tick,_)\<close> affirm
@@ -487,8 +487,8 @@ proc swap:
                         using fee_growth_eq_0 kk4 kk9 the_\<phi>(30) the_\<phi>(33) apply auto[1]
                         by (smt (verit, ccfv_threshold) fee_growth_eq_0 kk4 kk9 the_\<phi>(20) the_\<phi>(33) tick_of_price) ;;
                   affirm unfolding \<Delta>growth_def apply auto
-                        using fee_factor_GT_0 fee_growth_always_ge_0 kk6 kk8 the_\<phi>(37) apply force
-                        using fee_factor_GT_0 fee_growth_always_ge_0 kk9 t0 by force ;;
+                        using fee_rate'_GT_0 fee_growth_always_ge_0 kk6 kk8 the_\<phi>(37) apply force
+                        using fee_rate'_GT_0 fee_growth_always_ge_0 kk9 t0 by force ;;
 
         \<medium_right_bracket>. ;;
 
@@ -501,7 +501,7 @@ proc swap:
 
       \<medium_right_bracket> for \<open>_ \<s>\<u>\<b>\<j> real_next_tick < MAX_TICK\<close> ..
       \<medium_left_bracket>
-        have zx1: \<open>  zeroForOne \<Longrightarrow> tick_of_price next_price \<le> j\<close> by (smt (verit, best) fee_range kk6 kk8 price_of_L0 price_of_tick swap_step_next_price_Gt the_\<phi>(16) the_\<phi>(20) the_\<phi>(25) the_\<phi>(26) the_\<phi>(29) tick_of_price tick_of_price_LE_mono x1) 
+        have zx1: \<open>  zeroForOne \<Longrightarrow> tick_of_price next_price \<le> j\<close> by (smt (verit, best) fee_rate_range kk6 kk8 price_of_L0 price_of_tick swap_step_next_price_Gt the_\<phi>(16) the_\<phi>(20) the_\<phi>(25) the_\<phi>(26) the_\<phi>(29) tick_of_price tick_of_price_LE_mono x1) 
         have zx2: \<open>\<not> zeroForOne \<Longrightarrow> j \<le> tick_of_price next_price\<close> by (smt (verit, best) kk9 t0 the_\<phi>(29) tick_of_price tick_of_price_LE_mono)
 
         have zz6: \<open>  zeroForOne \<Longrightarrow> tick_next \<le> tick_of_price next_price\<close> by (metis (full_types) kk6 price_of_L0 tick_of_price tick_of_price_LE_mono)
@@ -513,7 +513,7 @@ proc swap:
           getTickAtSqrtRatio ($price) affirm using dual_order.strict_trans kk2 price_of_L0 by blast ;;
             \<rightarrow> tick
       \<medium_right_bracket>. \<medium_left_bracket> ;; \<medium_right_bracket>. ;; is \<open>tick_of_price next_price\<close>
-          affirm by (smt (verit, best) fee_range kk7 swap_step_next_price_Le t0 the_\<phi>(18) the_\<phi>(22) the_\<phi>(27) the_\<phi>(28) the_\<phi>(31) tick_of_price zx1 zz7) ;;
+          affirm by (smt (verit, best) fee_rate_range kk7 swap_step_next_price_Le t0 the_\<phi>(18) the_\<phi>(22) the_\<phi>(27) the_\<phi>(28) the_\<phi>(31) tick_of_price zx1 zz7) ;;
 
         \<open>\<v>\<a>\<r>[\<v>\<a>\<r>_liquidity] _\<close> is \<open>L (tick_of_price next_price)\<close> affirm using zxx . ;; ;;
         shift_current_tick_\<Delta>[where j=\<open>tick_of_price next_price\<close> and \<Delta>=\<Delta>growth]
@@ -529,7 +529,7 @@ proc swap:
               using fee_growth_eq_0 kk4 kk9 the_\<phi>(31) the_\<phi>(34) apply auto[1]
               using fee_growth_eq_0 kk4 kk9 the_\<phi>(34) by blast ;;
               affirm unfolding \<Delta>growth_def
-              using fee_factor_GT_0 fee_growth_always_ge_0 kk6 kk8 kk9 t0 the_\<phi>(38) by auto 
+              using fee_rate'_GT_0 fee_growth_always_ge_0 kk6 kk8 kk9 t0 the_\<phi>(38) by auto 
       \<medium_right_bracket>. ;;
 
       define real2_next_tick where
@@ -568,13 +568,13 @@ proc swap:
         apply (smt (verit, best) add.commute kk6 p2 p3 price_of_L0 reserve_change_add_left the_\<phi>(21))
         using p2 p3 reserve_change_add_right the_\<phi>(2) the_\<phi>(21) by presburger
 
-      have Iv5: \<open>?growth' + \<Delta>growth = growth + fee_growth zeroForOne fee_factor L price next_price\<close>
+      have Iv5: \<open>?growth' + \<Delta>growth = growth + fee_growth zeroForOne fee_rate' L price next_price\<close>
         unfolding \<Delta>growth_def by (auto,
             smt (verit, del_insts) Iv2 ab_semigroup_add_class.add_ac(1) add.commute fee_growth_add_right kk8 price_of_L0 the_\<phi>(21),
             metis fee_growth_add_right group_cancel.add1 kk9 the_\<phi>(2) the_\<phi>(21))
         
       ;;
-      \<medium_right_bracket> using \<open>let _ = _ in _\<close> by (auto simp add: Iv1 Iv2 Iv3 Iv4 Iv5 Iv6 d2 add_divide_distrib distrib_right fee_factor_def)
+      \<medium_right_bracket> using \<open>let _ = _ in _\<close> by (auto simp add: Iv1 Iv2 Iv3 Iv4 Iv5 Iv6 d2 add_divide_distrib distrib_right)
     ;; affirm apply (auto simp add: \<phi> zero_prod_def)
     using the_\<phi>(16) apply fastforce
     using the_\<phi>(16) apply fastforce
@@ -589,36 +589,36 @@ proc swap:
       is \<open>pool _ _ _ (L i') _ _ _\<close> affirm by auto ;;
 
   have \<open>zeroForOne \<Longrightarrow>
-    growth.map_fee0 (\<lambda>_. I_fee_growth_global (growth + fee_growth zeroForOne fee_factor L price price')) (gSum growth)
-      = gSum (growth + fee_growth zeroForOne fee_factor L price price')\<close>
+    growth.map_fee0 (\<lambda>_. I_fee_growth_global (growth + fee_growth zeroForOne fee_rate' L price price')) (gSum growth)
+      = gSum (growth + fee_growth zeroForOne fee_rate' L price price')\<close>
     apply (auto simp add: prod_eq_iff growth.map_fee0_def I_fee_growth_global_def growth.fee0_def)
     by (metis fee_growth_is_0_when_zeroForOne growth.fee1_def the_\<phi>(1) the_\<phi>lemmata(6))
 
   have proto_fee': \<open>proto_fee' =
-    (if 0 < fee_proto then ((if zeroForOne then fst else snd) (reserve_change zeroForOne L price price')) * fee_factor / real fee_proto else 0)\<close>
-    by (smt (verit) fee_factor_def split_def the_\<phi>(16) times_divide_eq_right)
+    (if 0 < fee_proto then ((if zeroForOne then fst else snd) (reserve_change zeroForOne L price price')) * fee_rate' / real fee_proto else 0)\<close>
+    by (smt (verit) fee_rate'_def split_def the_\<phi>(16) times_divide_eq_right)
 
   have proto_fee'_LE0: \<open>0 \<le> proto_fee'\<close>
-    unfolding proto_fee' using \<open>0 < price\<close> fee_factor_GT_0 reserve_change'_LE_0' the_\<phi>(1) the_\<phi>(12) the_\<phi>lemmata(6) by force ;;
+    unfolding proto_fee' using \<open>0 < price\<close> fee_rate'_GT_0 reserve_change'_LE_0' the_\<phi>(1) the_\<phi>(12) the_\<phi>lemmata(6) by force ;;
 
   if \<open>$zeroForOne\<close> \<medium_left_bracket>
     set_pool_fee_growth_0 ($fee_growth_global)
-    is \<open>pool _ _ _ _ (gSum (growth + fee_growth zeroForOne fee_factor L price price')) _ _\<close>
+    is \<open>pool _ _ _ _ (gSum (growth + fee_growth zeroForOne fee_rate' L price price')) _ _\<close>
     affirm by (auto simp add: prod_eq_iff growth.map_fee0_def I_fee_growth_global_def growth.fee0_def growth.fee1_def the_\<phi>(15)) (metis fee_growth_is_0_when_zeroForOne growth.fee1_def the_\<phi>(1) the_\<phi>(15) the_\<phi>(18)) ;;
 
-    if \<open>$protocolFee > 0\<close> \<medium_left_bracket> set_pool_protocal_fee_0 (\<open>fst (pool.protocal_fees _) + $protocolFee\<close>) \<medium_right_bracket>. \<medium_left_bracket> \<medium_right_bracket>. ;;
+    if \<open>$protocolFee > 0\<close> \<medium_left_bracket> set_pool_protocal_fee_0 (\<open>fst (pool.protocol_fees _) + $protocolFee\<close>) \<medium_right_bracket>. \<medium_left_bracket> \<medium_right_bracket>. ;;
 
    \<medium_right_bracket>. \<medium_left_bracket>
     set_pool_fee_growth_1 ($fee_growth_global)
-    is \<open>pool _ _ _ _ (gSum (growth + fee_growth zeroForOne fee_factor L price price')) _ _\<close>
+    is \<open>pool _ _ _ _ (gSum (growth + fee_growth zeroForOne fee_rate' L price price')) _ _\<close>
     affirm by (auto simp add: prod_eq_iff growth.map_fee1_def I_fee_growth_global_def growth.fee0_def growth.fee1_def the_\<phi>(15)) (metis \<open>0 < price\<close> fee_growth_is_0_when_not_zeroForOne growth.fee0_def the_\<phi>(15) the_\<phi>(18))  ;;
 
-    if \<open>$protocolFee > 0\<close> \<medium_left_bracket> set_pool_protocal_fee_1 (\<open>snd (pool.protocal_fees _) + $protocolFee\<close>) \<medium_right_bracket>. \<medium_left_bracket> \<medium_right_bracket>. ;;
+    if \<open>$protocolFee > 0\<close> \<medium_left_bracket> set_pool_protocal_fee_1 (\<open>snd (pool.protocol_fees _) + $protocolFee\<close>) \<medium_right_bracket>. \<medium_left_bracket> \<medium_right_bracket>. ;;
 
   \<medium_right_bracket>.
-  is \<open>pool price' i' False (L i') (gSum (growth + fee_growth zeroForOne fee_factor L price price')) fee_protocol
-           (protocal_fees + \<Delta>protocal_fees fee_protocol zeroForOne L price price' fee_factor)\<close>
-  affirm apply (cases protocal_fees; auto simp add: \<Delta>protocal_fees_def fee_proto_def proto_fee' zero_prod_def)
+  is \<open>pool price' i' False (L i') (gSum (growth + fee_growth zeroForOne fee_rate' L price price')) fee_protocol
+           (protocol_fees + \<Delta>protocal_fees fee_protocol zeroForOne L price price' fee_rate')\<close>
+  affirm apply (cases protocol_fees; auto simp add: \<Delta>protocal_fees_def fee_proto_def proto_fee' zero_prod_def)
     using fee_proto_def proto_fee' proto_fee'_LE0 zero_prod_def apply fastforce
     using fee_proto_def proto_fee' proto_fee'_LE0 zero_prod_def apply fastforce
     using fee_proto_def proto_fee' proto_fee'_LE0 apply force
@@ -629,12 +629,12 @@ proc swap:
       \<medium_left_bracket> \<open>$amount_specified - $amount_remaining\<close>, $amount_calculated \<medium_right_bracket>.
       \<medium_left_bracket> $amount_calculated, \<open>$amount_specified - $amount_remaining\<close> \<medium_right_bracket>. \<rightarrow> val amount0, amount1 ;;
   
-  $amount0 is \<open>if zeroForOne then fst (reserve_change' L price' price) / (1 - fee)
+  $amount0 is \<open>if zeroForOne then fst (reserve_change' L price' price) / (1 - fee_rate)
                     else - fst (reserve_change' L price price')\<close>
   affirm by (auto; insert the_\<phi>(16), force) ;; \<rightarrow> val amount0
 
   $amount1 is \<open>if zeroForOne then - snd (reserve_change' L price' price)
-                    else snd (reserve_change' L price price') / (1 - fee)\<close>
+                    else snd (reserve_change' L price price') / (1 - fee_rate)\<close>
   affirm by (auto; insert the_\<phi>(16), force) ;; \<rightarrow> val amount1
 
   if \<open>$zeroForOne\<close> \<medium_left_bracket>
@@ -645,22 +645,22 @@ proc swap:
         using the_\<phi>(15) apply blast
         using the_\<phi>(15) by force ;;
 
-    $amount0 is \<open>fst (reserve_change' L price' price) / (1 - fee)\<close>
+    $amount0 is \<open>fst (reserve_change' L price' price) / (1 - fee_rate)\<close>
   \<medium_right_bracket>. \<medium_left_bracket>
     if \<open>$amount0 < 0\<close> \<medium_left_bracket> \<open>-$amount0\<close> \<medium_right_bracket>. \<medium_left_bracket> \<open>0 \<Ztypecolon> \<real>\<close> \<medium_right_bracket>.
     is \<open>fst (reserve_change' L price price')\<close>
     affirm by (auto simp add: the_\<phi>(15)) (smt (verit) \<open>0 < price\<close> reserve_change'_LE_0' the_\<phi>(12) the_\<phi>(15) the_\<phi>lemmata(6)) ;;
 
-    $amount1 is \<open>snd (reserve_change' L price price') / (1 - fee)\<close>
+    $amount1 is \<open>snd (reserve_change' L price price') / (1 - fee_rate)\<close>
   \<medium_right_bracket>. ;;
 
   set_pool_unlock (\<open>True\<close>)
-  note [[ML_print_depth = 1000]]
+
   \<medium_right_bracket> apply (auto simp add: \<phi>)
-    apply (smt (verit, best) \<open>(if zeroForOne = (0 < amount_specified) then amount_specified - amount_remaining' else amount_calculated') = (if zeroForOne then fst (reserve_change' L price' price) / (1 - fee) else - fst (reserve_change' L price price'))\<close> fee_range nonzero_divide_eq_eq the_\<phi>lemmata(8))
-    using \<open>(if zeroForOne = (0 < amount_specified) then amount_calculated' else amount_specified - amount_remaining') = (if zeroForOne then - snd (reserve_change' L price' price) else snd (reserve_change' L price price') / (1 - fee))\<close> the_\<phi>lemmata(8) apply force
-    using \<open>(if zeroForOne = (0 < amount_specified) then amount_calculated' else amount_specified - amount_remaining') = (if zeroForOne then - snd (reserve_change' L price' price) else snd (reserve_change' L price price') / (1 - fee))\<close> \<open>0 \<noteq> amount_specified \<and> 0 < price_limit\<close> the_\<phi>lemmata(8) apply force
-    using \<open>(if zeroForOne = (0 < amount_specified) then amount_specified - amount_remaining' else amount_calculated') = (if zeroForOne then fst (reserve_change' L price' price) / (1 - fee) else - fst (reserve_change' L price price'))\<close> the_\<phi>lemmata(8) by force .
+    apply (smt (verit, best) \<open>(if zeroForOne = (0 < amount_specified) then amount_specified - amount_remaining' else amount_calculated') = (if zeroForOne then fst (reserve_change' L price' price) / (1 - fee_rate) else - fst (reserve_change' L price price'))\<close> fee_rate_range nonzero_divide_eq_eq the_\<phi>lemmata(8))
+    using \<open>(if zeroForOne = (0 < amount_specified) then amount_calculated' else amount_specified - amount_remaining') = (if zeroForOne then - snd (reserve_change' L price' price) else snd (reserve_change' L price price') / (1 - fee_rate))\<close> the_\<phi>lemmata(8) apply force
+    using \<open>(if zeroForOne = (0 < amount_specified) then amount_calculated' else amount_specified - amount_remaining') = (if zeroForOne then - snd (reserve_change' L price' price) else snd (reserve_change' L price price') / (1 - fee_rate))\<close> \<open>0 \<noteq> amount_specified \<and> 0 < price_limit\<close> the_\<phi>lemmata(8) apply force
+    using \<open>(if zeroForOne = (0 < amount_specified) then amount_specified - amount_remaining' else amount_calculated') = (if zeroForOne then fst (reserve_change' L price' price) / (1 - fee_rate) else - fst (reserve_change' L price price'))\<close> the_\<phi>lemmata(8) by force .
 
 end
 
